chore(na): Move test examples into own file

theories/rust_typing/existentials_na.v
@@ -136,862 +136,489 @@ End na_ex.
 
 Notation "'∃na;' P ',' τ" := (na_ex_plain_t _ _ P τ) (at level 40) : stdpp_scope.
 
-Section generated_code.
-  From refinedrust Require Import typing.
-
-  Section UnsafeCell_sls.
-    Context `{!typeGS Σ}.
-
-    Definition UnsafeCell_sls : struct_layout_spec := mk_sls "UnsafeCell" [
-      ("value", IntSynType I32)] StructReprTransparent.
-    Definition UnsafeCell_st : syn_type := UnsafeCell_sls.
-  End UnsafeCell_sls.
-
-  Section Cell_sls.
-    Context `{!typeGS Σ}.
-
-    Definition Cell_sls  : struct_layout_spec := mk_sls "Cell" [
-      ("value", UnsafeCell_st)] StructReprRust.
-    Definition Cell_st  : syn_type := Cell_sls .
-  End Cell_sls.
-
-  Section code.
-    Context `{!typeGS Σ}.
-    Open Scope printing_sugar.
-
-    Definition UnsafeCell_new_def : function := {|
-      f_args := [
-        ("value", (it_layout I32) : layout)
-      ];
-      f_local_vars := [
-        ("__0", (use_layout_alg' (UnsafeCell_st)) : layout);
-        ("__2", (it_layout I32) : layout)
-      ];
-      f_code :=
-        <[
-        "_bb0" :=
-        "__2" <-{ IntOp I32 } use{ IntOp I32 } ("value");
-        "__0" <-{ (use_op_alg' (UnsafeCell_st)) } StructInit UnsafeCell_sls [("value", use{ IntOp I32 } ("__2") : expr)];
-        return (use{ (use_op_alg' (UnsafeCell_st)) } ("__0"))
-        ]>%E $
-        ∅;
-      f_init := "_bb0";
-    |}.
-
-    Definition UnsafeCell_into_inner_def : function := {|
-      f_args := [
-        ("self", (use_layout_alg' (UnsafeCell_st)) : layout)
-      ];
-      f_local_vars := [
-        ("__0", (it_layout I32) : layout)
-      ];
-      f_code :=
-        <[
-        "_bb0" :=
-        "__0" <-{ IntOp I32 } use{ IntOp I32 } (("self") at{ UnsafeCell_sls } "value");
-        return (use{ IntOp I32 } ("__0"))
-        ]>%E $
-        ∅;
-      f_init := "_bb0";
-    |}.
-
-    Definition UnsafeCell_get_old_def : function := {|
-      f_args := [
-        ("self", void* : layout)
-      ];
-      f_local_vars := [
-        ("__0", (it_layout I32) : layout)
-      ];
-      f_code :=
-        <[
-        "_bb0" :=
-        annot: CopyLftNameAnnot "plft3" "ulft__";
-        "__0" <-{ IntOp I32 } use{ IntOp I32 } ((!{ PtrOp } ( "self" )) at{ (UnsafeCell_sls) } "value");
-        return (use{ IntOp I32 } ("__0"))
-        ]>%E $
-        ∅;
-      f_init := "_bb0";
-    |}.
-
-    Definition UnsafeCell_get_def : function := {|
-      f_args := [
-        ("self", void* : layout)
-      ];
-      f_local_vars := [
-        ("__0", void* : layout);
-        ("__2", void* : layout);
-        ("__3", void* : layout)
-      ];
-      f_code :=
-        <[
-        "_bb0" :=
-        annot: CopyLftNameAnnot "plft3" "ulft_1";
-        "__3" <-{ PtrOp } &raw{ Shr } (!{ PtrOp } ( "self" ));
-        "__2" <-{ PtrOp } use{ PtrOp } ("__3");
-        "__0" <-{ PtrOp } use{ PtrOp } ("__2");
-        return (use{ PtrOp } ("__0"))
-        ]>%E $
-        ∅;
-      f_init := "_bb0";
-    |}.
-
-    Definition Cell_new_def (UnsafeCell_new_loc : loc) : function := {|
-      f_args := [
-        ("value", (it_layout I32) : layout)
-      ];
-      f_local_vars := [
-        ("__0", (use_layout_alg' (Cell_st)) : layout);
-        ("__2", (use_layout_alg' (UnsafeCell_st)) : layout);
-        ("__3", (it_layout I32) : layout)
-      ];
-      f_code :=
-        <[
-        "_bb0" :=
-        "__3" <-{ IntOp I32 } use{ IntOp I32 } ("value");
-        "__2" <-{ (use_op_alg' (UnsafeCell_st)) } CallE UnsafeCell_new_loc [] [@{expr} use{ IntOp I32 } ("__3")];
-        Goto "_bb1"
-        ]>%E $
-        <[
-        "_bb1" :=
-        "__0" <-{ (use_op_alg' (Cell_st)) } StructInit Cell_sls [("value", use{ (use_op_alg' (UnsafeCell_st)) } ("__2") : expr)];
-        return (use{ (use_op_alg' (Cell_st)) } ("__0"))
-        ]>%E $
-        ∅;
-      f_init := "_bb0";
-    |}.
-
-    Definition Cell_into_inner_def (UnsafeCell_into_inner_loc : loc) : function := {|
-      f_args := [
-        ("self", (use_layout_alg' (Cell_st)) : layout)
-      ];
-      f_local_vars := [
-        ("__0", (it_layout I32) : layout);
-        ("__2", (use_layout_alg' (UnsafeCell_st)) : layout)
-      ];
-      f_code :=
-        <[
-        "_bb0" :=
-        "__2" <-{ (use_op_alg' (UnsafeCell_st)) } use{ (use_op_alg' (UnsafeCell_st)) } (("self") at{ Cell_sls } "value");
-        "__0" <-{ IntOp I32 } CallE UnsafeCell_into_inner_loc [] [@{expr} use{ (use_op_alg' (UnsafeCell_st)) } ("__2")];
-        Goto "_bb1"
-        ]>%E $
-        <[
-        "_bb1" :=
-        return (use{ IntOp I32 } ("__0"))
-        ]>%E $
-        ∅;
-      f_init := "_bb0";
-    |}.
-
-  End code.
-
-  Section UnsafeCell_ty.
-    Context `{!typeGS Σ}.
-
-    Definition UnsafeCell_ty : type (plist place_rfn [Z : Type]).
-    Proof using  Type*. exact (struct_t UnsafeCell_sls +[(int I32)]). Defined.
-
-    Definition UnsafeCell_rt : Type.
-    Proof using . let __a := eval hnf in (rt_of UnsafeCell_ty) in exact __a. Defined.
-
-    Global Typeclasses Transparent UnsafeCell_ty.
-    Global Typeclasses Transparent UnsafeCell_rt.
- End UnsafeCell_ty.
- Global Arguments UnsafeCell_rt : clear implicits.
-
-  Section UnsafeCell_inv_t.
-    Context `{!typeGS Σ}.
-
-    Program Definition UnsafeCell_inv_t_inv_spec : na_ex_inv_def (UnsafeCell_rt) (Z) :=
-      na_mk_ex_inv_def
-        (λ π inner_rfn 'x, ⌜inner_rfn = -[#(x)]⌝ ∗ ⌜Zeven x⌝ ∗ True)%I
-        [] [].
-
-    Definition UnsafeCell_inv_t : type (Z) :=
-      na_ex_plain_t _ _ UnsafeCell_inv_t_inv_spec UnsafeCell_ty.
-
-    Definition UnsafeCell_inv_t_rt : Type.
-    Proof using. let __a := eval hnf in (rt_of UnsafeCell_inv_t) in exact __a. Defined.
-
-    Global Typeclasses Transparent UnsafeCell_inv_t.
-    Global Typeclasses Transparent UnsafeCell_inv_t_rt.
-  End UnsafeCell_inv_t.
-  Global Arguments UnsafeCell_inv_t_rt : clear implicits.
-
-  Section Cell_ty.
-    Context `{!typeGS Σ}.
-
-    Definition Cell_ty : type (plist place_rfn [UnsafeCell_inv_t_rt : Type]).
-    Proof using  Type*. exact (struct_t Cell_sls +[UnsafeCell_inv_t]). Defined.
-    Definition Cell_rt : Type.
-    Proof using . let __a := eval hnf in (rt_of Cell_ty) in exact __a. Defined.
-
-    Global Typeclasses Transparent Cell_ty.
-    Global Typeclasses Transparent Cell_rt.
-  End Cell_ty.
-  Global Arguments Cell_rt : clear implicits.
-
-  Section Cell_inv_t.
-    Context `{!typeGS Σ}.
-
-    Program Definition Cell_inv_t_inv_spec : na_ex_inv_def (Cell_rt) (Z) :=
-      na_mk_ex_inv_def
-        (λ π inner_rfn 'x, ⌜inner_rfn = -[#(x)]⌝ ∗ ⌜Zeven x⌝ ∗ True)%I
-        [] [].
-
-    Definition Cell_inv_t : type (Z) :=
-      na_ex_plain_t _ _ Cell_inv_t_inv_spec Cell_ty.
-
-    Definition Cell_inv_t_rt : Type.
-    Proof using . let __a := eval hnf in (rt_of Cell_inv_t) in exact __a. Defined.
-
-    Global Typeclasses Transparent Cell_inv_t.
-    Global Typeclasses Transparent Cell_inv_t_rt.
-  End Cell_inv_t.
-  Global Arguments Cell_inv_t_rt : clear implicits.
-
-  Section specs.
-    Context `{!typeGS Σ}.
-
-    Definition type_of_UnsafeCell_new  :=
-      fn(∀ (()) : 0 | (x) : (Z), (λ ϝ, []); x @ (int I32); (λ π : thread_id, (⌜Zeven x⌝)))
-        → ∃ _ : unit, x @ UnsafeCell_inv_t; (λ π : thread_id, True).
-
-    Definition type_of_UnsafeCell_into_inner  :=
-      fn(∀ (()) : 0 | (x) : (Z), (λ ϝ, []); x @ UnsafeCell_inv_t; (λ π : thread_id, True))
-        → ∃ _ : unit, x @ (int I32); (λ π : thread_id, (⌜Zeven x⌝)).
-
-    Definition type_of_UnsafeCell_get_old  :=
-      fn(∀ ((), ulft__) : 1 | (x) : (_), (λ ϝ, []); #x @ (shr_ref UnsafeCell_inv_t ulft__); (λ π : thread_id, True))
-        → ∃ _ : unit, x @ (int I32); (λ π : thread_id, (⌜Zeven x⌝)).
-
-    Definition type_of_Cell_new  :=
-      fn(∀ (()) : 0 | (x) : (Z), (λ ϝ, []); x @ (int I32); (λ π : thread_id, (⌜Zeven x⌝)))
-        → ∃ _ : unit, x @ Cell_inv_t; (λ π : thread_id, True).
-
-    Definition type_of_Cell_into_inner  :=
-      fn(∀ (()) : 0 | (x) : (Z), (λ ϝ, []); x @ Cell_inv_t; (λ π : thread_id, True))
-        → ∃ _ : unit, x @ (int I32); (λ π : thread_id, (⌜Zeven x⌝)).
-  End specs.
-
-  Section proof.
-    Context `{!typeGS Σ}.
-
-    Definition UnsafeCell_new_lemma (π : thread_id) : Prop :=
-      syn_type_is_layoutable ((UnsafeCell_sls : syn_type)) →
-      ⊢ typed_function π (UnsafeCell_new_def ) [UnsafeCell_st; IntSynType I32] (type_of_UnsafeCell_new ).
-
-    Definition UnsafeCell_into_inner_lemma (π : thread_id) : Prop :=
-      syn_type_is_layoutable ((UnsafeCell_sls : syn_type)) →
-      ⊢ typed_function π (UnsafeCell_into_inner_def ) [IntSynType I32] (type_of_UnsafeCell_into_inner ).
-
-    Definition UnsafeCell_get_old_lemma (π : thread_id) : Prop :=
-      syn_type_is_layoutable (Cell_st) →
-      ⊢ typed_function π (UnsafeCell_get_old_def ) [IntSynType I32] (type_of_UnsafeCell_get_old ).
-
-    Definition Cell_new_lemma (π : thread_id) : Prop :=
-      ∀ (UnsafeCell_new_loc : loc) ,
-      syn_type_is_layoutable ((Cell_sls : syn_type)) →
-      syn_type_is_layoutable ((UnsafeCell_sls : syn_type)) →
-      UnsafeCell_new_loc ◁ᵥ{π} UnsafeCell_new_loc @ function_ptr [IntSynType I32] (type_of_UnsafeCell_new ) -∗
-      typed_function π (Cell_new_def UnsafeCell_new_loc  ) [Cell_st; UnsafeCell_st; IntSynType I32] (type_of_Cell_new ).
-  End proof.
-
-  Ltac UnsafeCell_new_prelude :=
-    unfold UnsafeCell_new_lemma;
-    set (FN_NAME := FUNCTION_NAME "UnsafeCell_new");
-    intros;
-    iStartProof;
-    start_function "UnsafeCell_new" ( [] ) (  x );
-    set (loop_map := BB_INV_MAP (PolyNil));
-    intros arg_value local___0 local___2;
-    prepare_parameters ( x );
-    init_lfts (∅ );
-    init_tyvars ( ∅ ).
-
-  Ltac UnsafeCell_into_inner_prelude :=
-    unfold UnsafeCell_into_inner_lemma;
-    set (FN_NAME := FUNCTION_NAME "UnsafeCell_into_inner");
-    intros;
-    iStartProof;
-    start_function "UnsafeCell_into_inner" ( [] ) (  x );
-    set (loop_map := BB_INV_MAP (PolyNil));
-    intros arg_self local___0;
-    prepare_parameters ( x );
-    init_lfts (∅ );
-    init_tyvars ( ∅ ).
-
-  Ltac UnsafeCell_get_old_prelude :=
-    unfold UnsafeCell_get_old_lemma;
-    set (FN_NAME := FUNCTION_NAME "Cell_get");
-    intros;
-    iStartProof;
-    let ulft__ := fresh "ulft__" in
-    start_function "Cell_get" ( [ [] ulft__] ) (  x );
-    set (loop_map := BB_INV_MAP (PolyNil));
-    intros arg_self local___0;
-    prepare_parameters ( x );
-    init_lfts (named_lft_update "ulft__" ulft__ $ ∅ );
-    init_tyvars ( ∅ ).
-
-  Ltac Cell_new_prelude :=
-    unfold Cell_new_lemma;
-    set (FN_NAME := FUNCTION_NAME "Cell_new");
-    intros;
-    iStartProof;
-    start_function "Cell_new" ( [] ) (  x );
-    set (loop_map := BB_INV_MAP (PolyNil));
-    intros arg_value local___0 local___2 local___3;
-    prepare_parameters ( x );
-    init_lfts (∅ );
-    init_tyvars ( ∅ ).
-
-  (* === V TYPING RULES V === *)
-
-  Section na_subtype.
-    Context `{!typeGS Σ}.
-    Context {rt X : Type} `{!Inhabited X} (P : na_ex_inv_def rt X).
-
-    Lemma owned_subtype_na_ex_plain_t π E L (ty : type rt) (r : rt) (r' : X) T :
-      (prove_with_subtype E L false ProveDirect (P.(na_inv_P) π r r') (λ L1 _ R, R -∗ T L1))
-      ⊢ owned_subtype π E L false r r' ty (∃na; P, ty) T.
-    Proof.
-      unfold owned_subtype, prove_with_subtype.
-
-      (* Nothing has changed *)
-      iIntros "HT".
-      iIntros (????) "#CTX #HE HL".
-      iMod ("HT" with "[//] [//] [//] CTX HE HL") as "(%L2 & % & %R2 & >(Hinv & HR2) & HL & HT)".
-      iExists L2. iFrame. iPoseProof ("HT" with "HR2") as "$". iModIntro.
-      iSplitR; last iSplitR.
-      - simpl. iPureIntro.
-        intros ly1 ly2 Hly1 HLy2. f_equiv. by eapply syn_type_has_layout_inj.
-      - simpl. eauto.
-      - iIntros (v) "Hv0".
-        iEval (rewrite /ty_own_val/=).
-        eauto with iFrame.
-    Qed.
-
-    Global Instance owned_subtype_na_ex_plain_t_inst π E L (ty : type rt) (r : rt) (r' : X) :
-      OwnedSubtype π E L false r r' ty (∃na; P, ty) :=
-      λ T, i2p (owned_subtype_na_ex_plain_t π E L ty r r' T).
-
-    Lemma na_ex_plain_t_open_owned F π (ty : type rt) (wl : bool) (l : loc) (x : X) :
-      lftE ⊆ F →
-      l ◁ₗ[π, Owned wl] PlaceIn x @ (◁ (∃na; P, ty)) ={F}=∗
-      ∃ r : rt, P.(na_inv_P) π r x ∗
-      l ◁ₗ[π, Owned false] PlaceIn r @ (◁ ty) ∗
-      (∀ rt' (lt' : ltype rt') (r' : place_rfn rt'),
-        l ◁ₗ[π, Owned false] r' @ lt' -∗
-        ⌜ltype_st lt' = ty_syn_type ty⌝ -∗
-        l ◁ₗ[π, Owned wl] r' @
-          (OpenedLtype lt' (◁ ty) (◁ ∃na; P, ty)
-            (λ (r : rt) (x : X), P.(na_inv_P) π r x)
-            (λ r x, True)))%I.
-    Proof.
-      (* Nothing has changed *)
-      iIntros (?) "Hb".
-      rewrite ltype_own_ofty_unfold /lty_of_ty_own.
-      iDestruct "Hb" as "(%ly & %Halg & %Hly & #Hsc & #Hlb & Hcred & %x' & Hrfn & Hb)".
-      iMod (maybe_use_credit with "Hcred Hb") as "(Hcred & Hat & Hb)"; first done.
-
-      unfold ty_own_val, na_ex_plain_t at 2.
-      iDestruct "Hb" as "(%v & Hl & %r & HP & Hv)".
-
-      iDestruct "Hrfn" as "<-".
-      iModIntro. iExists r. iFrame.
-      iSplitL "Hl Hv".
-      { rewrite ltype_own_ofty_unfold /lty_of_ty_own.
-        iExists ly. iFrame "#%". iSplitR; first done.
-        iExists r. iSplitR; first done. iModIntro. eauto with iFrame. }
-
-      iIntros (rt' lt' r') "Hb %Hst".
-      rewrite ltype_own_opened_unfold /opened_ltype_own.
-      iExists ly. rewrite Hst.
-      do 5 iR; iFrame.
-
-      clear -Halg Hly.
-      iApply (logical_step_intro_maybe with "Hat").
-      iIntros "Hcred' !>".
-      iIntros (r' r'' κs) "HP".
-      iSplitR; first done.
-      iIntros "Hdead Hl".
-      rewrite ltype_own_ofty_unfold /lty_of_ty_own.
-      iDestruct "Hl" as "(%ly' & _ & _ & Hsc' & _ & _ & %r0 & -> & >Hb)".
-      iDestruct "Hb" as "(%v' & Hl & Hv)".
-      iMod ("HP" with "Hdead" ) as "HP".
-      iModIntro.
-      rewrite ltype_own_core_equiv. simp_ltypes.
-      rewrite ltype_own_ofty_unfold /lty_of_ty_own.
-      iExists ly. simpl. iFrame "#%". iFrame.
-      iExists r''. iSplitR; first done. iModIntro.
-      iExists v'. iFrame. iExists r0. by iFrame.
-    Qed.
-
-    Lemma typed_place_na_ex_plain_t_owned π E L l (ty : type rt) x wl bmin K T :
-      (∀ r, introduce_with_hooks E L (P.(na_inv_P) π r x)
-        (λ L2, typed_place π E L2 l
-                (OpenedLtype (◁ ty) (◁ ty) (◁ (∃na; P, ty)) (λ (r : rt) (x : X), P.(na_inv_P) π r x) (λ r x, True))
-                (#r) bmin (Owned wl) K
-          (λ L2 κs li b2 bmin' rti ltyi ri strong weak,
-            (* no weak update possible - after all, we have just opened this invariant *)
-            T L2 κs li b2 bmin' rti ltyi ri strong None)))
-      ⊢ typed_place π E L l (◁ (∃na; P, ty))%I (#x) bmin (Owned wl) K T.
-    Proof.
-      unfold introduce_with_hooks, typed_place.
-
-      (* Nothing has changed *)
-      iIntros "HT". iIntros (F ???) "#CTX #HE HL Hincl Hb Hcont".
-      iApply fupd_place_to_wp.
-      iMod (na_ex_plain_t_open_owned with "Hb") as "(%r & HP & Hb & Hcl)"; first done.
-      iPoseProof ("Hcl" with "Hb []") as "Hb"; first done.
-      iMod ("HT" with "[] HE HL HP") as "(%L2 & HL & HT)"; first done.
-      iApply ("HT" with "[//] [//] CTX HE HL Hincl Hb").
-      iModIntro. iIntros (L' κs l2 b2 bmin0 rti ltyi ri strong weak) "Hincl Hl Hc".
-      iApply ("Hcont" with "Hincl Hl").
-      iSplit; last done.
-      iDestruct "Hc" as "[Hc _]".
-      destruct strong; last done.
-      simp_ltypes. done.
-    Qed.
-
-    Global Instance na_typed_place_ex_plain_t_owned_inst π E L l (ty : type rt) x wl bmin K `{!TCDone (K ≠ [])} :
-      TypedPlace E L π l (◁ (∃na; P, ty))%I #x bmin (Owned wl) K | 15 :=
-      λ T, i2p (typed_place_na_ex_plain_t_owned π E L l ty x wl bmin K T).
-
-
-    Lemma opened_na_ltype_acc_owned π {rt_cur rt_inner} (lt_cur : ltype rt_cur) (lt_inner : ltype rt_inner) Cpre Cpost l wl r :
-      l ◁ₗ[π, Owned wl] r @ OpenedNaLtype lt_cur lt_inner Cpre Cpost -∗
-      l ◁ₗ[π, Owned false] r @ lt_cur ∗
-      (∀ rt_cur' (lt_cur' : ltype rt_cur') r',
-        l ◁ₗ[π, Owned false] r' @ lt_cur' -∗
-        ⌜ltype_st lt_cur' = ltype_st lt_cur⌝ -∗
-        l ◁ₗ[π, Owned wl] r' @ OpenedNaLtype lt_cur' lt_inner Cpre Cpost).
-    Proof.
-      (* Nothing has changed *)
-
-      rewrite ltype_own_opened_na_unfold /opened_na_ltype_own.
-      iIntros "(%ly & ? & ? & ? & ? & $ & Hcl)".
-      iIntros (rt_cur' lt_cur' r') "Hown %Hst".
-      rewrite ltype_own_opened_na_unfold /opened_ltype_own.
-      iExists ly. rewrite Hst. eauto with iFrame.
-    Qed.
-
-    Lemma typed_place_opened_na_owned π E L {rt_cur rt_inner} (lt_cur : ltype rt_cur) (lt_inner : ltype rt_inner) Cpre Cpost r bmin0 l wl P''' T :
-      typed_place π E L l lt_cur r bmin0 (Owned false) P''' (λ L' κs l2 b2 bmin rti ltyi ri strong weak,
-        T L' κs l2 b2 bmin rti ltyi ri
-          (option_map (λ strong, mk_strong strong.(strong_rt)
-            (λ rti2 ltyi2 ri2, OpenedNaLtype (strong.(strong_lt) _ ltyi2 ri2) lt_inner Cpre Cpost)
-            (λ rti2 ri2, strong.(strong_rfn) _ ri2)
-            strong.(strong_R)) strong)
-          (* no weak access possible -- we currently don't have the machinery to restore and fold invariants at this point, though we could in principle enable this *)
-          None)
-      ⊢ typed_place π E L l (OpenedNaLtype lt_cur lt_inner Cpre Cpost) r bmin0 (Owned wl) P''' T.
-    Proof.
-      unfold introduce_with_hooks, typed_place.
-
-      (* Nothing has changed *)
-      iIntros "HT". iIntros (Φ F ??) "#CTX #HE HL #Hincl0 Hl HR".
-      iPoseProof (opened_na_ltype_acc_owned with "Hl") as "(Hl & Hcl)".
-      iApply ("HT" with "[//] [//] CTX HE HL [] Hl").
-      { destruct bmin0; done. }
-      iIntros (L' ??????? strong weak) "? Hl Hv".
-      iApply ("HR" with "[$] Hl").
-      iSplit; last done.
-      destruct strong as [ strong | ]; last done.
-      iIntros (???) "Hl Hst".
-      iDestruct "Hv" as "[Hv _]".
-      iMod ("Hv" with "Hl Hst") as "(Hl & %Hst & $)".
-      iPoseProof ("Hcl" with "Hl [//]") as "Hl".
-      cbn. eauto with iFrame.
-    Qed.
-
-    Global Instance typed_place_opened_na_owned_inst π E L {rt_cur rt_inner} (lt_cur : ltype rt_cur) (lt_inner : ltype rt_inner) Cpre Cpost r bmin0 l wl P :
-      TypedPlace E L π l (OpenedNaLtype lt_cur lt_inner Cpre Cpost) r bmin0 (Owned wl) P | 5 :=
-          λ T, i2p (typed_place_opened_na_owned π E L lt_cur lt_inner Cpre Cpost r bmin0 l wl P T).
-
-    Lemma na_ex_plain_t_open_shared E F π (ty : type rt) q κ l (x : X) :
-      lftE ⊆ E →
-      ↑shrN.@l ⊆ E →
-      (shr_locsE l 1 ⊆ F) →
-
-      lft_ctx -∗
-      na_own π F -∗
-      £ 1 -∗ (* Required: P.(na_inv_P) is not Timeless *)
-
-      q.[κ] -∗
-      l ◁ₗ[π, Shared κ] (#x) @ (◁ (∃na; P, ty)) ={E}=∗
-
-      ∃ r : rt,
-        P.(na_inv_P) π r x ∗
-        (l ◁ₗ[π, Owned false] (#r) @ (◁ ty)) ∗
-        &na{κ,π,shrN.@l} (∃ r' : rt, l ↦: ty_own_val ty π r' ∗ na_inv_P P π r' x) ∗
-
-        ( ∀ r' : rt,
-            l ◁ₗ[π, Owned false] #r' @ (◁ ty) ∗ P.(na_inv_P) π r' x ={E}=∗
-            q.[κ] ∗ na_own π F ).
-    Proof.
-      iIntros (???) "#LFT Hna Hcred Hq #Hb".
-      iEval (rewrite ltype_own_ofty_unfold /lty_of_ty_own) in "Hb".
-      iDestruct "Hb" as (ly Halg Hly) "(Hsc & Hlb & %v & -> & #Hb)".
-
-      iMod (fupd_mask_mono with "Hb") as "#Hb'"; first done; iClear "Hb".
-      iEval (unfold ty_shr, na_ex_plain_t) in "Hb'".
-      iDestruct "Hb'" as "(Hscr & Hbor & %ly' & %Hly' & %Halg')".
-
-      iMod (na_bor_acc with "LFT Hbor Hq Hna") as "((%r & Hl & HP) & Hna & Hvs)"; [ set_solver.. |].
-      iApply (lc_fupd_add_later with "Hcred").
-
-      do 2 iModIntro; iExists r; iFrame.
+Section na_subtype.
+  Context `{!typeGS Σ}.
+  Context {rt X : Type} `{!Inhabited X} (P : na_ex_inv_def rt X).
+
+  Lemma owned_subtype_na_ex_plain_t π E L (ty : type rt) (r : rt) (r' : X) T :
+    (prove_with_subtype E L false ProveDirect (P.(na_inv_P) π r r') (λ L1 _ R, R -∗ T L1))
+    ⊢ owned_subtype π E L false r r' ty (∃na; P, ty) T.
+  Proof.
+    unfold owned_subtype, prove_with_subtype.
+
+    (* Nothing has changed *)
+    iIntros "HT".
+    iIntros (????) "#CTX #HE HL".
+    iMod ("HT" with "[//] [//] [//] CTX HE HL") as "(%L2 & % & %R2 & >(Hinv & HR2) & HL & HT)".
+    iExists L2. iFrame. iPoseProof ("HT" with "HR2") as "$". iModIntro.
+    iSplitR; last iSplitR.
+    - simpl. iPureIntro.
+      intros ly1 ly2 Hly1 HLy2. f_equiv. by eapply syn_type_has_layout_inj.
+    - simpl. eauto.
+    - iIntros (v) "Hv0".
+      iEval (rewrite /ty_own_val/=).
+      eauto with iFrame.
+  Qed.
+
+  Global Instance owned_subtype_na_ex_plain_t_inst π E L (ty : type rt) (r : rt) (r' : X) :
+    OwnedSubtype π E L false r r' ty (∃na; P, ty) :=
+    λ T, i2p (owned_subtype_na_ex_plain_t π E L ty r r' T).
+
+  Lemma na_ex_plain_t_open_owned F π (ty : type rt) (wl : bool) (l : loc) (x : X) :
+    lftE ⊆ F →
+    l ◁ₗ[π, Owned wl] PlaceIn x @ (◁ (∃na; P, ty)) ={F}=∗
+    ∃ r : rt, P.(na_inv_P) π r x ∗
+    l ◁ₗ[π, Owned false] PlaceIn r @ (◁ ty) ∗
+    (∀ rt' (lt' : ltype rt') (r' : place_rfn rt'),
+      l ◁ₗ[π, Owned false] r' @ lt' -∗
+      ⌜ltype_st lt' = ty_syn_type ty⌝ -∗
+      l ◁ₗ[π, Owned wl] r' @
+        (OpenedLtype lt' (◁ ty) (◁ ∃na; P, ty)
+          (λ (r : rt) (x : X), P.(na_inv_P) π r x)
+          (λ r x, True)))%I.
+  Proof.
+    (* Nothing has changed *)
+    iIntros (?) "Hb".
+    rewrite ltype_own_ofty_unfold /lty_of_ty_own.
+    iDestruct "Hb" as "(%ly & %Halg & %Hly & #Hsc & #Hlb & Hcred & %x' & Hrfn & Hb)".
+    iMod (maybe_use_credit with "Hcred Hb") as "(Hcred & Hat & Hb)"; first done.
+
+    unfold ty_own_val, na_ex_plain_t at 2.
+    iDestruct "Hb" as "(%v & Hl & %r & HP & Hv)".
+
+    iDestruct "Hrfn" as "<-".
+    iModIntro. iExists r. iFrame.
+    iSplitL "Hl Hv".
+    { rewrite ltype_own_ofty_unfold /lty_of_ty_own.
+      iExists ly. iFrame "#%". iSplitR; first done.
+      iExists r. iSplitR; first done. iModIntro. eauto with iFrame. }
+
+    iIntros (rt' lt' r') "Hb %Hst".
+    rewrite ltype_own_opened_unfold /opened_ltype_own.
+    iExists ly. rewrite Hst.
+    do 5 iR; iFrame.
+
+    clear -Halg Hly.
+    iApply (logical_step_intro_maybe with "Hat").
+    iIntros "Hcred' !>".
+    iIntros (r' r'' κs) "HP".
+    iSplitR; first done.
+    iIntros "Hdead Hl".
+    rewrite ltype_own_ofty_unfold /lty_of_ty_own.
+    iDestruct "Hl" as "(%ly' & _ & _ & Hsc' & _ & _ & %r0 & -> & >Hb)".
+    iDestruct "Hb" as "(%v' & Hl & Hv)".
+    iMod ("HP" with "Hdead" ) as "HP".
+    iModIntro.
+    rewrite ltype_own_core_equiv. simp_ltypes.
+    rewrite ltype_own_ofty_unfold /lty_of_ty_own.
+    iExists ly. simpl. iFrame "#%". iFrame.
+    iExists r''. iSplitR; first done. iModIntro.
+    iExists v'. iFrame. iExists r0. by iFrame.
+  Qed.
+
+  Lemma typed_place_na_ex_plain_t_owned π E L l (ty : type rt) x wl bmin K T :
+    (∀ r, introduce_with_hooks E L (P.(na_inv_P) π r x)
+      (λ L2, typed_place π E L2 l
+              (OpenedLtype (◁ ty) (◁ ty) (◁ (∃na; P, ty)) (λ (r : rt) (x : X), P.(na_inv_P) π r x) (λ r x, True))
+              (#r) bmin (Owned wl) K
+        (λ L2 κs li b2 bmin' rti ltyi ri strong weak,
+          (* no weak update possible - after all, we have just opened this invariant *)
+          T L2 κs li b2 bmin' rti ltyi ri strong None)))
+    ⊢ typed_place π E L l (◁ (∃na; P, ty))%I (#x) bmin (Owned wl) K T.
+  Proof.
+    unfold introduce_with_hooks, typed_place.
+
+    (* Nothing has changed *)
+    iIntros "HT". iIntros (F ???) "#CTX #HE HL Hincl Hb Hcont".
+    iApply fupd_place_to_wp.
+    iMod (na_ex_plain_t_open_owned with "Hb") as "(%r & HP & Hb & Hcl)"; first done.
+    iPoseProof ("Hcl" with "Hb []") as "Hb"; first done.
+    iMod ("HT" with "[] HE HL HP") as "(%L2 & HL & HT)"; first done.
+    iApply ("HT" with "[//] [//] CTX HE HL Hincl Hb").
+    iModIntro. iIntros (L' κs l2 b2 bmin0 rti ltyi ri strong weak) "Hincl Hl Hc".
+    iApply ("Hcont" with "Hincl Hl").
+    iSplit; last done.
+    iDestruct "Hc" as "[Hc _]".
+    destruct strong; last done.
+    simp_ltypes. done.
+  Qed.
+
+  Global Instance na_typed_place_ex_plain_t_owned_inst π E L l (ty : type rt) x wl bmin K `{!TCDone (K ≠ [])} :
+    TypedPlace E L π l (◁ (∃na; P, ty))%I #x bmin (Owned wl) K | 15 :=
+    λ T, i2p (typed_place_na_ex_plain_t_owned π E L l ty x wl bmin K T).
+
+
+  Lemma opened_na_ltype_acc_owned π {rt_cur rt_inner} (lt_cur : ltype rt_cur) (lt_inner : ltype rt_inner) Cpre Cpost l wl r :
+    l ◁ₗ[π, Owned wl] r @ OpenedNaLtype lt_cur lt_inner Cpre Cpost -∗
+    l ◁ₗ[π, Owned false] r @ lt_cur ∗
+    (∀ rt_cur' (lt_cur' : ltype rt_cur') r',
+      l ◁ₗ[π, Owned false] r' @ lt_cur' -∗
+      ⌜ltype_st lt_cur' = ltype_st lt_cur⌝ -∗
+      l ◁ₗ[π, Owned wl] r' @ OpenedNaLtype lt_cur' lt_inner Cpre Cpost).
+  Proof.
+    (* Nothing has changed *)
+
+    rewrite ltype_own_opened_na_unfold /opened_na_ltype_own.
+    iIntros "(%ly & ? & ? & ? & ? & $ & Hcl)".
+    iIntros (rt_cur' lt_cur' r') "Hown %Hst".
+    rewrite ltype_own_opened_na_unfold /opened_ltype_own.
+    iExists ly. rewrite Hst. eauto with iFrame.
+  Qed.
+
+  Lemma typed_place_opened_na_owned π E L {rt_cur rt_inner} (lt_cur : ltype rt_cur) (lt_inner : ltype rt_inner) Cpre Cpost r bmin0 l wl P''' T :
+    typed_place π E L l lt_cur r bmin0 (Owned false) P''' (λ L' κs l2 b2 bmin rti ltyi ri strong weak,
+      T L' κs l2 b2 bmin rti ltyi ri
+        (option_map (λ strong, mk_strong strong.(strong_rt)
+          (λ rti2 ltyi2 ri2, OpenedNaLtype (strong.(strong_lt) _ ltyi2 ri2) lt_inner Cpre Cpost)
+          (λ rti2 ri2, strong.(strong_rfn) _ ri2)
+          strong.(strong_R)) strong)
+        (* no weak access possible -- we currently don't have the machinery to restore and fold invariants at this point, though we could in principle enable this *)
+        None)
+    ⊢ typed_place π E L l (OpenedNaLtype lt_cur lt_inner Cpre Cpost) r bmin0 (Owned wl) P''' T.
+  Proof.
+    unfold introduce_with_hooks, typed_place.
+
+    (* Nothing has changed *)
+    iIntros "HT". iIntros (Φ F ??) "#CTX #HE HL #Hincl0 Hl HR".
+    iPoseProof (opened_na_ltype_acc_owned with "Hl") as "(Hl & Hcl)".
+    iApply ("HT" with "[//] [//] CTX HE HL [] Hl").
+    { destruct bmin0; done. }
+    iIntros (L' ??????? strong weak) "? Hl Hv".
+    iApply ("HR" with "[$] Hl").
+    iSplit; last done.
+    destruct strong as [ strong | ]; last done.
+    iIntros (???) "Hl Hst".
+    iDestruct "Hv" as "[Hv _]".
+    iMod ("Hv" with "Hl Hst") as "(Hl & %Hst & $)".
+    iPoseProof ("Hcl" with "Hl [//]") as "Hl".
+    cbn. eauto with iFrame.
+  Qed.
+
+  Global Instance typed_place_opened_na_owned_inst π E L {rt_cur rt_inner} (lt_cur : ltype rt_cur) (lt_inner : ltype rt_inner) Cpre Cpost r bmin0 l wl P :
+    TypedPlace E L π l (OpenedNaLtype lt_cur lt_inner Cpre Cpost) r bmin0 (Owned wl) P | 5 :=
+        λ T, i2p (typed_place_opened_na_owned π E L lt_cur lt_inner Cpre Cpost r bmin0 l wl P T).
+
+  Lemma na_ex_plain_t_open_shared E F π (ty : type rt) q κ l (x : X) :
+    lftE ⊆ E →
+    ↑shrN.@l ⊆ E →
+    (shr_locsE l 1 ⊆ F) →
+
+    lft_ctx -∗
+    na_own π F -∗
+    £ 1 -∗ (* Required: P.(na_inv_P) is not Timeless *)
+
+    q.[κ] -∗
+    l ◁ₗ[π, Shared κ] (#x) @ (◁ (∃na; P, ty)) ={E}=∗
+
+    ∃ r : rt,
+      P.(na_inv_P) π r x ∗
+      (l ◁ₗ[π, Owned false] (#r) @ (◁ ty)) ∗
+      &na{κ,π,shrN.@l} (∃ r' : rt, l ↦: ty_own_val ty π r' ∗ na_inv_P P π r' x) ∗
+
+      ( ∀ r' : rt,
+          l ◁ₗ[π, Owned false] #r' @ (◁ ty) ∗ P.(na_inv_P) π r' x ={E}=∗
+          q.[κ] ∗ na_own π F ).
+  Proof.
+    iIntros (???) "#LFT Hna Hcred Hq #Hb".
+    iEval (rewrite ltype_own_ofty_unfold /lty_of_ty_own) in "Hb".
+    iDestruct "Hb" as (ly Halg Hly) "(Hsc & Hlb & %v & -> & #Hb)".
+
+    iMod (fupd_mask_mono with "Hb") as "#Hb'"; first done; iClear "Hb".
+    iEval (unfold ty_shr, na_ex_plain_t) in "Hb'".
+    iDestruct "Hb'" as "(Hscr & Hbor & %ly' & %Hly' & %Halg')".
+
+    iMod (na_bor_acc with "LFT Hbor Hq Hna") as "((%r & Hl & HP) & Hna & Hvs)"; [ set_solver.. |].
+    iApply (lc_fupd_add_later with "Hcred").
+
+    do 2 iModIntro; iExists r; iFrame.
+
+    iSplitL "Hl".
+    { rewrite ltype_own_ofty_unfold /lty_of_ty_own.
+      iExists ly => /=.
+      iFrame (Halg Hly) "Hlb Hscr"; iR.
+      iExists r; iR.
+      by iModIntro. }
+
+    iR; iIntros (r') "(Hl & HP)".
+    iEval (rewrite ltype_own_ofty_unfold /lty_of_ty_own) in "Hl".
+    iDestruct "Hl" as (???) "(_ & _ & _ & (% & <- & Hl)) /=".
+    iMod (fupd_mask_mono with "Hl") as "Hl"; first solve_ndisj.
+
+    iApply ("Hvs" with "[Hl HP] Hna").
+    iExists r'; iFrame.
+  Qed.
+
+  Lemma na_own_split π E E' :
+    E' ⊆ E ->
+    na_own π E -∗ na_own π E' ∗ na_own π (E ∖ E').
+  Proof.
+    iIntros (?) "Hna".
+    rewrite comm.
+
+    iApply na_own_union.
+    { set_solver. }
+
+    replace E with ((E ∖ E') ∪ E') at 1; first done.
+
+    set_unfold.
+    split; first intuition.
+    destruct (decide (x ∈ E')); intuition.
+  Qed.
+
+  Lemma typed_place_na_ex_plain_t_shared π E L l (ty : type rt) x κ bmin K T :
+    find_in_context (FindNaOwn) (λ '(π', mask),
+      ⌜π = π'⌝ ∗
+      ⌜↑shrN.@l ⊆ mask⌝ ∗
+      prove_with_subtype E L false ProveDirect (£ 1) (λ L1 _ R, R -∗
+        li_tactic (lctx_lft_alive_count_goal E L1 κ) (λ '(κs, L2),
+          ∀ r, introduce_with_hooks E L2
+            (P.(na_inv_P) π r x ∗
+            l ◁ₗ[π, Owned false] (#r) @
+              (OpenedNaLtype (◁ ty) (◁ ty)
+                (λ rfn, P.(na_inv_P) π rfn x)
+                (λ _, na_own π (↑shrN.@l) ∗ llft_elt_toks κs)) ∗
+            na_own π (mask ∖ ↑shrN.@l))
+            (λ L3,
+              typed_place π E L3 l
+                (ShadowedLtype (AliasLtype _ (ty_syn_type ty) l) #tt (◁ (∃na; P, ty)))
+                (#x) (bmin ⊓ₖ Shared κ) (Shared κ) K
+                (λ L4 κs li b2 bmin' rti ltyi ri strong weak,
+                  T L4 κs li b2 bmin' rti ltyi ri strong None)))))
+    ⊢ typed_place π E L l (◁ (∃na; P, ty))%I (#x) bmin (Shared κ) K T.
+  Proof.
+    rewrite /find_in_context.
+    iDestruct 1 as ([π' mask]) "(Hna & <- & % & HT) /=".
+
+    rewrite /typed_place /introduce_with_hooks.
+    iIntros (Φ ???) "#(LFT & TIME & LLCTX) #HE HL ? Hl Hcont".
+
+    rewrite /prove_with_subtype.
+    iApply fupd_place_to_wp.
+
+    iMod ("HT" with "[] [] [] [$LFT $TIME $LLCTX] HE HL")
+        as "(% & % & % & >(Hcred & HR) & HL & HT)"; [ done.. |].
+    iSpecialize ("HT" with "HR").
+
+    rewrite /li_tactic /lctx_lft_alive_count_goal.
+    iDestruct "HT" as (???) "HT".
+
+    iMod (fupd_mask_subseteq (lftE ∪ shrE)) as "Hf"; first done.
+    iMod (lctx_lft_alive_count_tok with "HE HL") as (q) "(Htok & Htokcl & HL)"; [ solve_ndisj.. |].
+    iPoseProof (na_own_split with "Hna") as "(Hna & Hna')"; first done.
+    iMod (na_ex_plain_t_open_shared with "LFT Hna Hcred Htok Hl") as (r) "(HP & Hl & #Hbor & Hvs)"; [ try solve_ndisj.. |].
+
+    iEval (rewrite ltype_own_ofty_unfold /lty_of_ty_own) in "Hl".
+    iDestruct "Hl" as (ly Halg Hly) "(#Hsc & #Hlb & _ & (% & <- & Hl))".
+
+    iMod ("HT" with "[] HE HL [$HP Hl Htokcl Hvs Hna']") as "HT"; first solve_ndisj.
+    { rewrite ltype_own_opened_na_unfold /opened_na_ltype_own.
+      iFrame.
+      iExists ly; repeat iR.
 
       iSplitL "Hl".
       { rewrite ltype_own_ofty_unfold /lty_of_ty_own.
-        iExists ly => /=.
-        iFrame (Halg Hly) "Hlb Hscr"; iR.
-        iExists r; iR.
-        by iModIntro. }
-
-      iR; iIntros (r') "(Hl & HP)".
-      iEval (rewrite ltype_own_ofty_unfold /lty_of_ty_own) in "Hl".
-      iDestruct "Hl" as (???) "(_ & _ & _ & (% & <- & Hl)) /=".
-      iMod (fupd_mask_mono with "Hl") as "Hl"; first solve_ndisj.
-
-      iApply ("Hvs" with "[Hl HP] Hna").
-      iExists r'; iFrame.
-    Qed.
-
-    Lemma na_own_split π E E' :
-      E' ⊆ E ->
-      na_own π E -∗ na_own π E' ∗ na_own π (E ∖ E').
-    Proof.
-      iIntros (?) "Hna".
-      rewrite comm.
-
-      iApply na_own_union.
-      { set_solver. }
-
-      replace E with ((E ∖ E') ∪ E') at 1; first done.
-
-      set_unfold.
-      split; first intuition.
-      destruct (decide (x ∈ E')); intuition.
-    Qed.
-
-    Lemma typed_place_na_ex_plain_t_shared π E L l (ty : type rt) x κ bmin K T :
-      find_in_context (FindNaOwn) (λ '(π', mask),
-        ⌜π = π'⌝ ∗
-        ⌜↑shrN.@l ⊆ mask⌝ ∗
-        prove_with_subtype E L false ProveDirect (£ 1) (λ L1 _ R, R -∗
-          li_tactic (lctx_lft_alive_count_goal E L1 κ) (λ '(κs, L2),
-            ∀ r, introduce_with_hooks E L2
-              (P.(na_inv_P) π r x ∗
-              l ◁ₗ[π, Owned false] (#r) @
-                (OpenedNaLtype (◁ ty) (◁ ty)
-                  (λ rfn, P.(na_inv_P) π rfn x)
-                  (λ _, na_own π (↑shrN.@l) ∗ llft_elt_toks κs)) ∗
-              na_own π (mask ∖ ↑shrN.@l))
-              (λ L3,
-                typed_place π E L3 l
-                  (ShadowedLtype (AliasLtype _ (ty_syn_type ty) l) #tt (◁ (∃na; P, ty)))
-                  (#x) (bmin ⊓ₖ Shared κ) (Shared κ) K
-                  (λ L4 κs li b2 bmin' rti ltyi ri strong weak,
-                    T L4 κs li b2 bmin' rti ltyi ri strong None)))))
-      ⊢ typed_place π E L l (◁ (∃na; P, ty))%I (#x) bmin (Shared κ) K T.
-    Proof.
-      rewrite /find_in_context.
-      iDestruct 1 as ([π' mask]) "(Hna & <- & % & HT) /=".
-
-      rewrite /typed_place /introduce_with_hooks.
-      iIntros (Φ ???) "#(LFT & TIME & LLCTX) #HE HL ? Hl Hcont".
-
-      rewrite /prove_with_subtype.
-      iApply fupd_place_to_wp.
-
-      iMod ("HT" with "[] [] [] [$LFT $TIME $LLCTX] HE HL")
-          as "(% & % & % & >(Hcred & HR) & HL & HT)"; [ done.. |].
-      iSpecialize ("HT" with "HR").
-
-      rewrite /li_tactic /lctx_lft_alive_count_goal.
-      iDestruct "HT" as (???) "HT".
-
-      iMod (fupd_mask_subseteq (lftE ∪ shrE)) as "Hf"; first done.
-      iMod (lctx_lft_alive_count_tok with "HE HL") as (q) "(Htok & Htokcl & HL)"; [ solve_ndisj.. |].
-      iPoseProof (na_own_split with "Hna") as "(Hna & Hna')"; first done.
-      iMod (na_ex_plain_t_open_shared with "LFT Hna Hcred Htok Hl") as (r) "(HP & Hl & #Hbor & Hvs)"; [ try solve_ndisj.. |].
-
-      iEval (rewrite ltype_own_ofty_unfold /lty_of_ty_own) in "Hl".
-      iDestruct "Hl" as (ly Halg Hly) "(#Hsc & #Hlb & _ & (% & <- & Hl))".
-
-      iMod ("HT" with "[] HE HL [$HP Hl Htokcl Hvs Hna']") as "HT"; first solve_ndisj.
-      { rewrite ltype_own_opened_na_unfold /opened_na_ltype_own.
-        iFrame.
         iExists ly; repeat iR.
+        by iExists r; iR. }
 
-        iSplitL "Hl".
-        { rewrite ltype_own_ofty_unfold /lty_of_ty_own.
-          iExists ly; repeat iR.
-          by iExists r; iR. }
+      iApply logical_step_intro.
 
-        iApply logical_step_intro.
+      iIntros (r') "Hinv Hl".
+      iEval (rewrite ltype_own_ofty_unfold /lty_of_ty_own) in "Hl".
+      iDestruct "Hl" as (ly' Halg' Hly') "(_ & #Hlb' & _ & (% & <- & Hl))".
 
-        iIntros (r') "Hinv Hl".
-        iEval (rewrite ltype_own_ofty_unfold /lty_of_ty_own) in "Hl".
-        iDestruct "Hl" as (ly' Halg' Hly') "(_ & #Hlb' & _ & (% & <- & Hl))".
-
-        iMod ("Hvs" with "[Hl Hinv]") as "(? & ?)".
-        { iFrame.
-          rewrite ltype_own_ofty_unfold /lty_of_ty_own.
-          iExists ly'; repeat iR.
-          by iExists r'; iR. }
-
-        iFrame.
-        by iApply "Htokcl". }
-
-      iDestruct "HT" as (?) "(HL & HT)".
-
-      iApply ("HT" with "[//] [//] [$LFT $TIME $LLCTX] HE HL [] []").
-      { iApply bor_kind_min_incl_r. }
-      { rewrite ltype_own_shadowed_unfold /shadowed_ltype_own.
-
-        iR; iSplitL.
-        { rewrite ltype_own_alias_unfold /alias_lty_own.
-          iExists ly. by repeat iR. }
-
+      iMod ("Hvs" with "[Hl Hinv]") as "(? & ?)".
+      { iFrame.
         rewrite ltype_own_ofty_unfold /lty_of_ty_own.
-        iExists ly; repeat iR.
-        iExists x; repeat iR.
+        iExists ly'; repeat iR.
+        by iExists r'; iR. }
 
-        rewrite /ty_shr /na_ex_plain_t.
-        repeat iR.
-        by iExists ly; repeat iR. }
+      iFrame.
+      by iApply "Htokcl". }
 
-      iMod "Hf" as "_".
-      iIntros "!>" (? ? ? ? ? ? ? ? strong ?) "Hincl Hl [ Hstrong _ ]".
+    iDestruct "HT" as (?) "(HL & HT)".
 
-      iApply ("Hcont" with "Hincl Hl").
-      destruct strong; iSplit; [| done.. ].
-      by simp_ltypes.
-    Qed.
+    iApply ("HT" with "[//] [//] [$LFT $TIME $LLCTX] HE HL [] []").
+    { iApply bor_kind_min_incl_r. }
+    { rewrite ltype_own_shadowed_unfold /shadowed_ltype_own.
 
-    Global Instance typed_place_na_ex_plain_t_shared_inst π E L l (ty : type rt) x κ bmin K `{!TCDone (K ≠ [])} :
-      TypedPlace E L π l (◁ (∃na; P, ty))%I #x bmin (Shared κ) K | 15 :=
-      λ T, i2p (typed_place_na_ex_plain_t_shared π E L l ty x κ bmin K T).
+      iR; iSplitL.
+      { rewrite ltype_own_alias_unfold /alias_lty_own.
+        iExists ly. by repeat iR. }
 
-    Lemma typed_place_alias_shared π E L l l2 rt''' (r : place_rfn rt''') st bmin0 κ P''' T :
-      find_in_context (FindLoc l2) (λ '(existT rt2 (lt2, r2, b2, π2)),
-        ⌜π = π2⌝ ∗
-        typed_place π E L l2 lt2 r2 b2 b2 P''' (λ L' κs li b3 bmin rti ltyi ri strong weak,
-          T L' κs li b3 bmin rti ltyi ri
-            (fmap (λ strong, mk_strong (λ _, _) (λ _ _ _, AliasLtype rt''' st l2) (λ _ _, r)
-              (* give back ownership through R *)
-              (λ rti2 ltyi2 ri2, l2 ◁ₗ[π, b2] strong.(strong_rfn) _ ri2 @ strong.(strong_lt) _ ltyi2 ri2 ∗ strong.(strong_R) _ ltyi2 ri2)) strong)
-            None))
-      ⊢ typed_place π E L l (AliasLtype rt''' st l2) r bmin0 (Shared κ) P''' T.
-    Proof.
-      unfold find_in_context, typed_place.
+      rewrite ltype_own_ofty_unfold /lty_of_ty_own.
+      iExists ly; repeat iR.
+      iExists x; repeat iR.
 
-      iDestruct 1 as ((rt2 & (((lt & r''') & b2) & π2))) "(Hl2 & <- & HP)". simpl.
-      iIntros (????) "#CTX #HE HL #Hincl Hl Hcont".
-      rewrite ltype_own_alias_unfold /alias_lty_own.
-      iDestruct "Hl" as "(%ly & % & -> & #? & #?)".
+      rewrite /ty_shr /na_ex_plain_t.
+      repeat iR.
+      by iExists ly; repeat iR. }
 
-      iApply ("HP" with "[//] [//] CTX HE HL [] Hl2").
-      { iApply bor_kind_incl_refl. }
-      iIntros (L' κs l2 b0 bmin rti ltyi ri strong weak) "#Hincl1 Hl2 Hcl HT HL".
-      iApply ("Hcont" with "[//] Hl2 [Hcl] HT HL").
+    iMod "Hf" as "_".
+    iIntros "!>" (? ? ? ? ? ? ? ? strong ?) "Hincl Hl [ Hstrong _ ]".
 
-      iSplit; last done.
+    iApply ("Hcont" with "Hincl Hl").
+    destruct strong; iSplit; [| done.. ].
+    by simp_ltypes.
+  Qed.
 
-      destruct strong as [ strong |]; last done.
-      iDestruct "Hcl" as "[Hcl _]"; simpl.
+  Global Instance typed_place_na_ex_plain_t_shared_inst π E L l (ty : type rt) x κ bmin K `{!TCDone (K ≠ [])} :
+    TypedPlace E L π l (◁ (∃na; P, ty))%I #x bmin (Shared κ) K | 15 :=
+    λ T, i2p (typed_place_na_ex_plain_t_shared π E L l ty x κ bmin K T).
 
-      iIntros (rti2 ltyi2 ri2) "Hl2 %Hst".
-      iMod ("Hcl" with "Hl2 [//]") as "(Hl & % & Hstrong)".
+  Lemma typed_place_alias_shared π E L l l2 rt''' (r : place_rfn rt''') st bmin0 κ P''' T :
+    find_in_context (FindLoc l2) (λ '(existT rt2 (lt2, r2, b2, π2)),
+      ⌜π = π2⌝ ∗
+      typed_place π E L l2 lt2 r2 b2 b2 P''' (λ L' κs li b3 bmin rti ltyi ri strong weak,
+        T L' κs li b3 bmin rti ltyi ri
+          (fmap (λ strong, mk_strong (λ _, _) (λ _ _ _, AliasLtype rt''' st l2) (λ _ _, r)
+            (* give back ownership through R *)
+            (λ rti2 ltyi2 ri2, l2 ◁ₗ[π, b2] strong.(strong_rfn) _ ri2 @ strong.(strong_lt) _ ltyi2 ri2 ∗ strong.(strong_R) _ ltyi2 ri2)) strong)
+          None))
+    ⊢ typed_place π E L l (AliasLtype rt''' st l2) r bmin0 (Shared κ) P''' T.
+  Proof.
+    unfold find_in_context, typed_place.
+
+    iDestruct 1 as ((rt2 & (((lt & r''') & b2) & π2))) "(Hl2 & <- & HP)". simpl.
+    iIntros (????) "#CTX #HE HL #Hincl Hl Hcont".
+    rewrite ltype_own_alias_unfold /alias_lty_own.
+    iDestruct "Hl" as "(%ly & % & -> & #? & #?)".
+
+    iApply ("HP" with "[//] [//] CTX HE HL [] Hl2").
+    { iApply bor_kind_incl_refl. }
+    iIntros (L' κs l2 b0 bmin rti ltyi ri strong weak) "#Hincl1 Hl2 Hcl HT HL".
+    iApply ("Hcont" with "[//] Hl2 [Hcl] HT HL").
+
+    iSplit; last done.
+
+    destruct strong as [ strong |]; last done.
+    iDestruct "Hcl" as "[Hcl _]"; simpl.
+
+    iIntros (rti2 ltyi2 ri2) "Hl2 %Hst".
+    iMod ("Hcl" with "Hl2 [//]") as "(Hl & % & Hstrong)".
+    iModIntro.
+
+    rewrite ltype_own_alias_unfold /alias_lty_own.
+    iFrame. iSplit; [| done].
+    iExists ly; by repeat iR.
+  Qed.
+  Global Instance typed_place_alias_shared_inst π E L l l2 rt r st bmin0 κ P :
+    TypedPlace E L π l (AliasLtype rt st l2) r bmin0 (Shared κ) P :=
+    λ T, i2p (typed_place_alias_shared π E L l l2 rt r st bmin0 κ P T).
+
+  Lemma stratify_ltype_alias_shared π E L mu mdu ma {M} (m : M) l l2 rt''' st r κ (T : stratify_ltype_cont_t) :
+    ( if decide (ma = StratNoRefold)
+      then
+        T L True _ (AliasLtype rt''' st l2) r
+      else
+        find_in_context (FindLoc l2) (λ '(existT rt2 (lt2, r2, b2, π2)),
+          ⌜π = π2⌝ ∗ ⌜ltype_st lt2 = st⌝ ∗ ⌜b2 = Owned false⌝ ∗
+          (* recursively stratify *)
+          stratify_ltype π E L mu mdu ma m l2 lt2 r2 b2
+            (λ L2 R rt2' lt2' r2',
+                (T L2 ((l2 ◁ₗ[π, Owned false] r2' @ lt2') ∗ R) rt''' (AliasLtype rt''' st l2) r))))
+    ⊢ stratify_ltype π E L mu mdu ma m l (AliasLtype rt''' st l2) r (Shared κ) T.
+  Proof.
+    rewrite /stratify_ltype /find_in_context.
+    iIntros "HT".
+
+    destruct (decide (ma = StratNoRefold)) as [-> | ].
+    { iIntros (????) "#CTX #HE HL Hl". iModIntro. iExists _, _, _, _, _. iFrame.
+      iSplitR; first done. iApply logical_step_intro. by iFrame. }
+
+    iDestruct "HT" as ([rt2 [[[lt2 r2] b2] π2]]) "(Hl2 & <- & <- & -> & HT)"; simpl.
+
+    iIntros (????) "#CTX #HE HL Hl".
+    rewrite ltype_own_alias_unfold /alias_lty_own.
+    simp_ltypes.
+
+    iDestruct "Hl" as "(%ly & %Halg & -> & %Hly & Hlb)".
+
+    iMod ("HT" with "[//] [//] [//] CTX HE HL Hl2") as (L3 R rt2' lt2' r2') "(HL & %Hst & Hstep & HT)".
+    iModIntro. iExists _, _, _, _, _.
+    iFrame; iR.
+
+    iApply (logical_step_compose with "Hstep").
+    iApply logical_step_intro.
+    iIntros "($ & $)".
+
+    rewrite ltype_own_alias_unfold /alias_lty_own.
+    by iExists ly; iFrame.
+  Qed.
+  Global Instance stratify_ltype_alias_shared_inst π E L mu mdu ma {M} (m : M) l l2 rt st r κ :
+    StratifyLtype π E L mu mdu ma m l (AliasLtype rt st l2) r (Shared κ) :=
+    λ T, i2p (stratify_ltype_alias_shared π E L mu mdu ma m l l2 rt st r κ T).
+
+  Lemma stratify_ltype_opened_na_Owned {rt_cur rt_inner} π E L mu mdu ma {M} (ml : M) l
+      (lt_cur : ltype rt_cur) (lt_inner : ltype rt_inner)
+      (Cpre Cpost : rt_inner → iProp Σ) r (T : stratify_ltype_cont_t) :
+    stratify_ltype π E L mu mdu ma ml l lt_cur r (Owned false)
+      (λ L' R rt_cur' lt_cur' (r' : place_rfn rt_cur'),
+        if decide (ma = StratNoRefold)
+        then (* keep it open *)
+          T L' R _ (OpenedNaLtype lt_cur' lt_inner Cpre Cpost) r'
+        else (* fold the invariant *)
+          ∃ ri,
+            (* show that the core of lt_cur' is a subtype of lt_inner *)
+            weak_subltype E L' (Owned false) (r') (#ri) lt_cur' lt_inner (
+              (* re-establish the invariant *)
+              prove_with_subtype E L' true ProveDirect (Cpre ri)
+                (λ L'' _ R2, T L'' (Cpost ri ∗ R2 ∗ R) unit (AliasLtype unit (ltype_st lt_inner) l) #tt)))
+    ⊢ stratify_ltype π E L mu mdu ma ml l (OpenedNaLtype lt_cur lt_inner Cpre Cpost) r (Owned false) T.
+  Proof.
+    rewrite /stratify_ltype /weak_subltype /prove_with_subtype.
+
+    iIntros "Hstrat" (F ???) "#CTX #HE HL Hl".
+    rewrite ltype_own_opened_na_unfold /opened_na_ltype_own.
+
+    iDestruct "Hl" as "(%ly & %Halg & %Hly & #Hlb & %Hst & Hl & Hcl)".
+    iMod ("Hstrat" with "[//] [//] [//] CTX HE HL Hl") as "(%L2 & %R & %rt_cur' & %lt_cur' & %r' & HL & %Hst' & Hstep & HT)".
+
+    destruct (decide (ma = StratNoRefold)) as [-> | ].
+    - (* don't fold *)
       iModIntro.
-
-      rewrite ltype_own_alias_unfold /alias_lty_own.
-      iFrame. iSplit; [| done].
-      iExists ly; by repeat iR.
-    Qed.
-    Global Instance typed_place_alias_shared_inst π E L l l2 rt r st bmin0 κ P :
-      TypedPlace E L π l (AliasLtype rt st l2) r bmin0 (Shared κ) P :=
-      λ T, i2p (typed_place_alias_shared π E L l l2 rt r st bmin0 κ P T).
-
-    Lemma stratify_ltype_alias_shared π E L mu mdu ma {M} (m : M) l l2 rt''' st r κ (T : stratify_ltype_cont_t) :
-      ( if decide (ma = StratNoRefold)
-        then
-          T L True _ (AliasLtype rt''' st l2) r
-        else
-          find_in_context (FindLoc l2) (λ '(existT rt2 (lt2, r2, b2, π2)),
-            ⌜π = π2⌝ ∗ ⌜ltype_st lt2 = st⌝ ∗ ⌜b2 = Owned false⌝ ∗
-            (* recursively stratify *)
-            stratify_ltype π E L mu mdu ma m l2 lt2 r2 b2
-              (λ L2 R rt2' lt2' r2',
-                 (T L2 ((l2 ◁ₗ[π, Owned false] r2' @ lt2') ∗ R) rt''' (AliasLtype rt''' st l2) r))))
-      ⊢ stratify_ltype π E L mu mdu ma m l (AliasLtype rt''' st l2) r (Shared κ) T.
-    Proof.
-      rewrite /stratify_ltype /find_in_context.
-      iIntros "HT".
-
-      destruct (decide (ma = StratNoRefold)) as [-> | ].
-      { iIntros (????) "#CTX #HE HL Hl". iModIntro. iExists _, _, _, _, _. iFrame.
-        iSplitR; first done. iApply logical_step_intro. by iFrame. }
-
-      iDestruct "HT" as ([rt2 [[[lt2 r2] b2] π2]]) "(Hl2 & <- & <- & -> & HT)"; simpl.
-
-      iIntros (????) "#CTX #HE HL Hl".
-      rewrite ltype_own_alias_unfold /alias_lty_own.
-      simp_ltypes.
-
-      iDestruct "Hl" as "(%ly & %Halg & -> & %Hly & Hlb)".
-
-      iMod ("HT" with "[//] [//] [//] CTX HE HL Hl2") as (L3 R rt2' lt2' r2') "(HL & %Hst & Hstep & HT)".
-      iModIntro. iExists _, _, _, _, _.
-      iFrame; iR.
+      iExists _, _, _, _, _; iFrame; iR.
 
       iApply (logical_step_compose with "Hstep").
       iApply logical_step_intro.
-      iIntros "($ & $)".
+      iIntros "(Hl & $)".
 
-      rewrite ltype_own_alias_unfold /alias_lty_own.
-      by iExists ly; iFrame.
-    Qed.
-    Global Instance stratify_ltype_alias_shared_inst π E L mu mdu ma {M} (m : M) l l2 rt st r κ :
-      StratifyLtype π E L mu mdu ma m l (AliasLtype rt st l2) r (Shared κ) :=
-      λ T, i2p (stratify_ltype_alias_shared π E L mu mdu ma m l l2 rt st r κ T).
-
-    Lemma stratify_ltype_opened_na_Owned {rt_cur rt_inner} π E L mu mdu ma {M} (ml : M) l
-        (lt_cur : ltype rt_cur) (lt_inner : ltype rt_inner)
-        (Cpre Cpost : rt_inner → iProp Σ) r (T : stratify_ltype_cont_t) :
-      stratify_ltype π E L mu mdu ma ml l lt_cur r (Owned false)
-        (λ L' R rt_cur' lt_cur' (r' : place_rfn rt_cur'),
-          if decide (ma = StratNoRefold)
-          then (* keep it open *)
-            T L' R _ (OpenedNaLtype lt_cur' lt_inner Cpre Cpost) r'
-          else (* fold the invariant *)
-            ∃ ri,
-              (* show that the core of lt_cur' is a subtype of lt_inner *)
-              weak_subltype E L' (Owned false) (r') (#ri) lt_cur' lt_inner (
-                (* re-establish the invariant *)
-                prove_with_subtype E L' true ProveDirect (Cpre ri)
-                  (λ L'' _ R2, T L'' (Cpost ri ∗ R2 ∗ R) unit (AliasLtype unit (ltype_st lt_inner) l) #tt)))
-      ⊢ stratify_ltype π E L mu mdu ma ml l (OpenedNaLtype lt_cur lt_inner Cpre Cpost) r (Owned false) T.
-    Proof.
-      rewrite /stratify_ltype /weak_subltype /prove_with_subtype.
-
-      iIntros "Hstrat" (F ???) "#CTX #HE HL Hl".
       rewrite ltype_own_opened_na_unfold /opened_na_ltype_own.
+      iExists ly; iFrame.
+      rewrite -Hst'; do 3 iR.
+      done.
 
-      iDestruct "Hl" as "(%ly & %Halg & %Hly & #Hlb & %Hst & Hl & Hcl)".
-      iMod ("Hstrat" with "[//] [//] [//] CTX HE HL Hl") as "(%L2 & %R & %rt_cur' & %lt_cur' & %r' & HL & %Hst' & Hstep & HT)".
+    - (* fold it again *)
+      iDestruct "HT" as "(%ri & HT)".
+      iMod ("HT" with "[//] CTX HE HL") as "(Hincl & HL & HT)".
+      iMod ("HT" with "[//] [//] [//] CTX HE HL") as "(%L3 & %κs & %R2 & Hstep' & HL & HT)".
 
-      destruct (decide (ma = StratNoRefold)) as [-> | ].
-      - (* don't fold *)
-        iModIntro.
-        iExists _, _, _, _, _; iFrame; iR.
+      iExists L3, _, _, _, _; iFrame.
+      iSplitR.
+      { by simp_ltypes. }
 
-        iApply (logical_step_compose with "Hstep").
-        iApply logical_step_intro.
-        iIntros "(Hl & $)".
+      iApply logical_step_fupd.
+      iApply (logical_step_compose with "Hstep").
+      iPoseProof (logical_step_mask_mono with "Hcl") as "Hcl"; first done.
+      iApply (logical_step_compose with "Hcl").
+      iApply (logical_step_compose with "Hstep'").
+      iApply logical_step_intro.
 
-        rewrite ltype_own_opened_na_unfold /opened_na_ltype_own.
-        iExists ly; iFrame.
-        rewrite -Hst'; do 3 iR.
-        done.
+      iIntros "!> (Hpre & $) Hcl (Hl & $)".
+      iMod (ltype_incl_use with "Hincl Hl") as "Hl"; first done.
 
-      - (* fold it again *)
-        iDestruct "HT" as "(%ri & HT)".
-        iMod ("HT" with "[//] CTX HE HL") as "(Hincl & HL & HT)".
-        iMod ("HT" with "[//] [//] [//] CTX HE HL") as "(%L3 & %κs & %R2 & Hstep' & HL & HT)".
+      iPoseProof ("Hcl" with "Hpre Hl") as "Hvs".
+      iSplitL "".
+      { rewrite ltype_own_alias_unfold /alias_lty_own.
+        rewrite -Hst.
 
-        iExists L3, _, _, _, _; iFrame.
-        iSplitR.
-        { by simp_ltypes. }
+        by iExists ly; repeat iR. }
 
-        iApply logical_step_fupd.
-        iApply (logical_step_compose with "Hstep").
-        iPoseProof (logical_step_mask_mono with "Hcl") as "Hcl"; first done.
-        iApply (logical_step_compose with "Hcl").
-        iApply (logical_step_compose with "Hstep'").
-        iApply logical_step_intro.
+      iMod (fupd_mask_mono with "Hvs") as "Hvs"; first set_solver.
+      done.
+  Qed.
 
-        iIntros "!> (Hpre & $) Hcl (Hl & $)".
-        iMod (ltype_incl_use with "Hincl Hl") as "Hl"; first done.
+  Global Instance stratify_ltype_opened_na_owned_inst {rt_cur rt_inner} π E L mu mdu ma {M} (ml : M) l
+      (lt_cur : ltype rt_cur) (lt_inner : ltype rt_inner) (Cpre Cpost : rt_inner → iProp Σ) r:
+    StratifyLtype π E L mu mdu ma ml l (OpenedNaLtype lt_cur lt_inner Cpre Cpost) r (Owned false) := λ T, i2p (stratify_ltype_opened_na_Owned π E L mu mdu ma ml l lt_cur lt_inner Cpre Cpost r T).
 
-        iPoseProof ("Hcl" with "Hpre Hl") as "Hvs".
-        iSplitL "".
-        { rewrite ltype_own_alias_unfold /alias_lty_own.
-          rewrite -Hst.
-
-          by iExists ly; repeat iR. }
-
-        iMod (fupd_mask_mono with "Hvs") as "Hvs"; first set_solver.
-        done.
-    Qed.
-
-    Global Instance stratify_ltype_opened_na_owned_inst {rt_cur rt_inner} π E L mu mdu ma {M} (ml : M) l
-        (lt_cur : ltype rt_cur) (lt_inner : ltype rt_inner) (Cpre Cpost : rt_inner → iProp Σ) r:
-      StratifyLtype π E L mu mdu ma ml l (OpenedNaLtype lt_cur lt_inner Cpre Cpost) r (Owned false) := λ T, i2p (stratify_ltype_opened_na_Owned π E L mu mdu ma ml l lt_cur lt_inner Cpre Cpost r T).
-
-  End na_subtype.
-
-  (* === ^ TYPING RULES ^ === *)
-
-  Section proof.
-    Context `{!typeGS Σ}.
-
-    Lemma UnsafeCell_new_proof (π : thread_id) :
-      UnsafeCell_new_lemma π.
-    Proof.
-      UnsafeCell_new_prelude.
-
-      repeat liRStep; liShow.
-
-      all: print_remaining_goal.
-      Unshelve. all: sidecond_solver.
-      Unshelve. all: sidecond_hammer.
-      Unshelve. all: print_remaining_sidecond.
-    Qed.
-
-    Lemma UnsafeCell_into_inner_proof (π : thread_id) :
-      UnsafeCell_into_inner_lemma π.
-    Proof.
-      UnsafeCell_into_inner_prelude.
-
-      repeat liRStep; liShow.
-
-      all: print_remaining_goal.
-      Unshelve. all: sidecond_solver.
-      Unshelve. all: sidecond_hammer.
-      Unshelve. all: print_remaining_sidecond.
-    Qed.
-
-    Lemma Cell_new_proof (π : thread_id) :
-      Cell_new_lemma π.
-    Proof.
-      Cell_new_prelude.
-
-      repeat liRStep; liShow.
-
-      all: print_remaining_goal.
-      Unshelve. all: sidecond_solver.
-      Unshelve. all: sidecond_hammer.
-      Unshelve. all: print_remaining_sidecond.
-
-      (* NOTE: The QED takes a lot of time *)
-    Admitted.
-
-    Lemma UnsafeCell_get_old_proof (π : thread_id) :
-      UnsafeCell_get_old_lemma π.
-    Proof.
-      UnsafeCell_get_old_prelude.
-
-      repeat liRStep; liShow.
-
-      Unshelve. all: sidecond_solver.
-      Unshelve. all: sidecond_hammer.
-      Unshelve. all: print_remaining_sidecond.
-    Qed.
-  End proof.
-
-End generated_code.
+End na_subtype.
